klaas comments

src/lib/utils/DY.Lib.SplitFunction.fst
@@ -400,7 +400,18 @@ let rec memP_mk_dependent_tagged_local_funs #tag_set_t #local_fun_t l tag_set lo
     memP_mk_dependent_tagged_local_funs t tag_set local_fun
 
 /// Normalize pre-condition and post-conditions from correctness lemmas derived from `mk_global_fun_correct`
-/// to save some boilerplate when using this framework
+/// to save some boilerplate when using this framework.
+/// These correctness lemmas are generally instantiated with a concrete list of tag and local functions,
+/// they have as pre-condition something like `no_repeats_p (map fst tag_and_funs_list)`,
+/// which users prove by normalization,
+/// and they have as post-condition something like
+///     for_allP (has_local_fun global_fun) tag_and_funs_list
+/// which users want to normalize to obtain
+///     has_local_fun global_fun (tag_1, local_fun_1) /\
+///     ... /\
+///     has_local_fun global_fun (tag_n, local_fun_n)
+/// The function `do_split_boilerplate` takes care of applying these normalizations
+/// to correctness lemmas derived from `mk_global_fun_correct`.
 
 val get_fv_name: FStar.Tactics.term -> FStar.Tactics.Tac unit
 let get_fv_name t =
@@ -411,15 +422,17 @@ let get_fv_name t =
   )
   | _ -> fail ("get_fv_name: not a free variable: " ^ (term_to_string t))
 
-val do_boilerplate:
+val do_split_boilerplate:
   #a:Type ->
   #p:(a -> Type) -> #q:(a -> Type) ->
+  // the $ below ensures F* doesn't do subtyping during unification,
+  // which allows us to unify `p` and `q` precisely
   ($lem: (x: a -> Lemma (requires (p x)) (ensures (q x)))) ->
   x:a ->
   #[get_fv_name (quote x)] x_s:string ->
   #_:squash (norm [delta_only [x_s; `%List.Tot.no_repeats_p; `%List.Tot.memP; `%List.Tot.map; `%fst; `%dfst]; iota; zeta] (p x)) ->
   squash (norm [delta_only [x_s; `%for_allP]; iota; zeta] (q x))
-let do_boilerplate #a #p #q $lem x #x_s #_ =
+let do_split_boilerplate #a #p #q $lem x #x_s #_ =
   norm_spec [delta_only [x_s; `%List.Tot.no_repeats_p; `%List.Tot.memP; `%List.Tot.map; `%fst; `%dfst]; iota; zeta] (p x);
   lem x;
   norm_spec [delta_only [x_s; `%for_allP]; iota; zeta] (q x)
