examples/nsl_pk/DY.Example.NSL.Protocol.Stateful.Proof.fst
@@ -105,8 +105,8 @@ instance protocol_invariants_nsl: protocol_invariants = {
 
 /// Lemmas that the global state predicate contains all the local ones
 
-let _ = do_boilerplate mk_state_pred_correct all_sessions
-let _ = do_boilerplate mk_event_pred_correct all_events
+let _ = do_split_boilerplate mk_state_pred_correct all_sessions
+let _ = do_split_boilerplate mk_event_pred_correct all_events
 
 (*** Proofs ***)
 
